

# Linear Algebra Module 5 Assignment

$$1) A^{-1} = \begin{bmatrix} 7 & 8 \\ 1 & 2 \end{bmatrix}, (A^{-1})^{-1} = A = \frac{1}{2 \cdot 7 - 1 \cdot 8} \begin{bmatrix} 2 & -8 \\ -1 & 7 \end{bmatrix} = \begin{bmatrix} \frac{2}{6} & -\frac{8}{6} \\ -\frac{1}{6} & \frac{7}{6} \end{bmatrix} = \begin{bmatrix} \frac{1}{3} & -\frac{4}{3} \\ -\frac{1}{6} & \frac{7}{6} \end{bmatrix} \text{ in}$$

2) Suppose  $A$  is invertible.

a) from the supposition we get access to the Invertible Matrix Theorem, which tells us it is equivalent to  $(A^T)^{-1} = (A^{-1})^T$  from the properties of transposition. This tells us  $A^T$  is invertible. Now we know both matrices are invertible. Using the first circle of implication the supposition also entails that an invertible matrix is row equivalent to the Identity matrix. Thus, both  $A^T$  and  $A$  are equivalent to  $I_n$ , and so their product would be row equivalent to  $I_n$  (itself when reduced) as well, because there is no row operation being performed.  $A^T A$  implies the supposition that the product is invertible this way. This assumes  $A$  is an  $n \times n$  matrix.



2) b) Assuming  $A$  is  $n \times n$ , we can show that  $A^{-1} = (A^T A)^{-1} A^T$  through computation of the product of  $A$  and  $(A^T A)^{-1} A^T$  by assigning  $A$  but first let's do some algebra to show why:

$$A^{-1} = (A^T A)^{-1} A^T = A^{-1} (A^T)^{-1} A^T = A^{-1} I$$

$$A A^{-1} = A A^{-1} I$$

$$I = I I$$

$$I = I$$

and

$$A (A^T A)^{-1} A^T = A A^{-1} (A^T)^{-1} A^T = I I = I$$

So for  $A$  a  $2 \times 2$  matrix we can assign it the value of  $I_2: \begin{bmatrix} 1 & 0 \\ 0 & 1 \end{bmatrix}$  and compute; the computation goes in a circle, in both cases we start with  $I_2$  and end with  $I_2$ , they are equivalent statements.

$$(A^T A)^{-1} A^T = A (A^T A)^{-1} A^T.$$



3) The question is find the value of  $b$  for inverses:

$$A = \begin{bmatrix} 3 & -2 & -2 \\ -1 & 1 & 1 \\ 3 & -1 & -2 \end{bmatrix} \quad B = \begin{bmatrix} 1 & a & 0 \\ -1 & b & 1 \\ 2 & c & -1 \end{bmatrix}$$

In order to find the inverse of only one column we augment by only that column of  $I_n$ , and perform Gauss-Jordan.

So, working from  $A\bar{x} = \bar{e}_2$ , since the other columns can be found we find  $B_{22}$ :

$$\left[ \begin{array}{ccc|c} 3 & -2 & -2 & 0 \\ -1 & 1 & 1 & 1 \\ 3 & -1 & -2 & 0 \end{array} \right] \begin{array}{l} R_1 = R_1 + 2R_2 \\ R_3 = R_3 + R_2 \end{array} \left[ \begin{array}{ccc|c} 1 & 0 & 0 & 2 \\ -1 & 1 & 1 & 1 \\ 3 & -1 & -2 & 0 \end{array} \right]$$

$$\left[ \begin{array}{ccc|c} 1 & 0 & 0 & 2 \\ -1 & 1 & 1 & 1 \\ 2 & 0 & -1 & 1 \end{array} \right] \begin{array}{l} R_2 = R_2 + R_1 \\ R_3 = R_3 - 2R_1 \end{array} \left[ \begin{array}{ccc|c} 1 & 0 & 0 & 2 \\ 0 & 1 & 1 & 3 \\ 2 & 0 & -1 & 1 \end{array} \right]$$

$$\left[ \begin{array}{ccc|c} 1 & 0 & 0 & 2 \\ 0 & 1 & 1 & 3 \\ 0 & 0 & -1 & -3 \end{array} \right] \begin{array}{l} R_2 = R_2 + R_3 \\ R_3 = (-1)R_3 \end{array} \left[ \begin{array}{ccc|c} 1 & 0 & 0 & 2 \\ 0 & 1 & 0 & 0 \\ 0 & 0 & 1 & -3 \end{array} \right]$$

$$= \left[ \begin{array}{ccc|c} 1 & 0 & 0 & 2 \\ 0 & 1 & 0 & 0 \\ 0 & 0 & 1 & 3 \end{array} \right] \therefore b = 0.$$